src/Interpreter.v
@@ -13,37 +13,14 @@
 (* *********************************************************************)
 
 From Coq Require Import Streams List Syntax.
+From Coq.Program Require Import Equality.
+From Coq.ssr Require Import ssreflect.
 From MenhirLib Require Automaton.
 From MenhirLib Require Import Alphabet.
+From MenhirLib Require Import Validator_safe.
 
 Module Make(Import A:Automaton.T).
-
-(** The error monad **)
-Inductive result (A:Type) :=
-  | Err: result A
-  | OK: A -> result A.
-
-Arguments Err [A].
-Arguments OK [A].
-
-Definition bind {A B: Type} (f: result A) (g: A -> result B): result B :=
-  match f with
-    | OK x => g x
-    | Err => Err
-  end.
-
-Definition bind2 {A B C: Type} (f: result (A * B)) (g: A -> B -> result C):
-  result C :=
-  match f with
-    | OK (x, y) => g x y
-    | Err => Err
-  end.
-
-Notation "'do' X <- A ; B" := (bind A (fun X => B))
-  (at level 200, X ident, A at level 100, B at level 200).
-
-Notation "'do' ( X , Y ) <- A ; B" := (bind2 A (fun X Y => B))
-  (at level 200, X ident, Y ident, A at level 100, B at level 200).
+Module Import ValidSafe := Validator_safe.Make A.
 
 (** Some operations on streams **)
 
@@ -58,13 +35,7 @@ Infix "++" := app_str (right associativity, at level 60).
 
 Lemma app_str_app_assoc {A:Type} (l1 l2:list A) (s:Stream A) :
   l1 ++ (l2 ++ s) = (l1 ++ l2) ++ s.
-Proof.
-induction l1.
-reflexivity.
-simpl.
-rewrite IHl1.
-reflexivity.
-Qed.
+Proof. induction l1 as [|?? IH]=>//=. rewrite IH //. Qed.
 
 (** The type of a non initial state: the type of semantic values associated
    with the last symbol of this state. *)
@@ -76,7 +47,21 @@ Definition noninitstate_type state :=
     and a nested stack. **)
 Definition stack := list (sigT noninitstate_type). (* eg. list {state & state_type state} *)
 
-Section Init.
+Section Interpreter.
+
+Hypothesis safe: safe.
+
+(* Properties of the automaton deduced from safety validation. *)
+Proposition shift_head_symbs: shift_head_symbs.
+Proof. pose proof safe; unfold ValidSafe.safe in H; intuition. Qed.
+Proposition goto_head_symbs: goto_head_symbs.
+Proof. pose proof safe; unfold ValidSafe.safe in H; intuition. Qed.
+Proposition shift_past_state: shift_past_state.
+Proof. pose proof safe; unfold ValidSafe.safe in H; intuition. Qed.
+Proposition goto_past_state: goto_past_state.
+Proof. pose proof safe; unfold ValidSafe.safe in H; intuition. Qed.
+Proposition reduce_ok: reduce_ok.
+Proof. pose proof safe; unfold ValidSafe.safe in H; intuition. Qed.
 
 Variable init : initstate.
 
@@ -87,26 +72,129 @@ Definition state_of_stack (stack:stack): state :=
     | existT _ s _::_ => s
   end.
 
+(** The stack of states of an automaton stack **)
+Definition state_stack_of_stack (stack:stack) :=
+  (List.map
+    (fun cell:sigT noninitstate_type => singleton_state_pred (projT1 cell))
+    stack ++ [singleton_state_pred init])%list.
+
+(** The stack of symbols of an automaton stack **)
+Definition symb_stack_of_stack (stack:stack) :=
+  List.map
+    (fun cell:sigT noninitstate_type => last_symb_of_non_init_state (projT1 cell))
+    stack.
+
+(** The stack invariant : it basically states that the assumptions on the
+    states are true. **)
+Inductive stack_invariant: stack -> Prop :=
+  | stack_invariant_constr:
+    forall stack,
+      prefix      (head_symbs_of_state (state_of_stack stack))
+                  (symb_stack_of_stack stack) ->
+      prefix_pred (head_states_of_state (state_of_stack stack))
+                  (state_stack_of_stack stack) ->
+      stack_invariant_next stack ->
+      stack_invariant stack
+with stack_invariant_next: stack -> Prop :=
+  | stack_invariant_next_nil:
+      stack_invariant_next []
+  | stack_invariant_next_cons:
+    forall state_cur st stack_rec,
+      stack_invariant stack_rec ->
+      stack_invariant_next (existT _ state_cur st::stack_rec).
+
 (** [pop] pops some symbols from the stack. It returns the popped semantic
     values using [sem_popped] as an accumulator and discards the popped
     states.**)
-Fixpoint pop (symbols_to_pop:list symbol) (stack_cur:stack):
-  forall {A:Type} (action:arrows_right A (map symbol_semantic_type symbols_to_pop)),
-    result (stack * A) :=
-  match symbols_to_pop return forall {A:Type} (action:arrows_right A (map _ symbols_to_pop)), result (stack * A) with
-    | [] => fun A action => OK (stack_cur, action)
-    | t::q => fun A action =>
-      match stack_cur with
-        | existT _ state_cur sem::stack_rec =>
-          match compare_eqdec (last_symb_of_non_init_state state_cur) t with
-            | left e =>
-              let sem_conv := eq_rect _ symbol_semantic_type sem _ e in
-              pop q stack_rec (action sem_conv)
-            | right _ => Err
-          end
-        | [] => Err
-      end
-  end.
+Fixpoint pop (symbols_to_pop:list symbol) {A:Type} (stk:stack) :
+  prefix symbols_to_pop (symb_stack_of_stack stk) ->
+  forall (action:arrows_right A (map symbol_semantic_type symbols_to_pop)),
+    stack * A.
+unshelve refine
+  (match symbols_to_pop
+      return
+         prefix symbols_to_pop (symb_stack_of_stack stk) ->
+         forall (action:arrows_right A (map _ symbols_to_pop)), stack * A
+   with
+     | [] => fun _ action => (stk, action)
+     | t::q => fun Hp action =>
+       match stk
+          return prefix (t::q) (symb_stack_of_stack stk) -> stack * A
+       with
+         | existT _ state_cur sem::stack_rec => fun Hp =>
+           let sem_conv := eq_rect _ symbol_semantic_type sem _ _ in
+           pop q _ stack_rec _ (action sem_conv)
+         | [] => fun Hp => False_rect _ _
+       end Hp
+   end).
+Proof.
+  - simpl in Hp. clear -Hp. abstract now inversion Hp.
+  - simpl in Hp. clear -Hp. abstract now inversion Hp.
+  - simpl in Hp. clear -Hp. abstract now inversion Hp.
+Defined.
+
+(* Equivalent declarative specification for pop, so that we avoid
+   (part of) the dependent types nightmare. *)
+Inductive pop_spec {A:Type} :
+    forall (symbols_to_pop:list symbol) (stk : stack)
+           (action : arrows_right A (map symbol_semantic_type symbols_to_pop))
+           (stk' : stack) (sem : A),
+      Prop :=
+  | Nil_pop_spec stk sem : pop_spec [] stk sem stk sem
+  | Cons_pop_spec symbols_to_pop st stk action sem stk' res :
+      pop_spec symbols_to_pop stk (action sem) stk' res ->
+      pop_spec (last_symb_of_non_init_state st::symbols_to_pop)
+               (existT _ st sem :: stk) action stk' res.
+
+Lemma pop_spec_ok {A:Type} symbols_to_pop stk Hp action stk' res:
+  pop symbols_to_pop stk Hp action = (stk', res) <->
+  pop_spec (A:=A) symbols_to_pop stk action stk' res.
+Proof.
+  revert stk Hp action.
+  induction symbols_to_pop as [|t symbols_to_pop IH]=>stk Hp action /=.
+  - split.
+    + intros [= <- <-]. constructor.
+    + intros H. inversion H. simpl_existTs. by subst.
+  - destruct stk as [|[st sem]]=>/=; [by destruct pop_subproof0|].
+    destruct pop_subproof=>/=. rewrite IH. split.
+    + intros. by constructor.
+    + intros H. inversion H. simpl_existTs. by subst.
+Qed.
+
+
+Lemma pop_preserves_invariant symbols_to_pop stk Hp A action :
+  stack_invariant stk ->
+  stack_invariant (fst (pop symbols_to_pop stk Hp (A:=A) action)).
+Proof.
+  revert stk Hp A action. induction symbols_to_pop as [|t q IH]=>//=.
+  intros stk Hp A action Hi.
+  destruct Hi as [stack Hp' Hpp [|state st stk']].
+  - destruct pop_subproof0.
+  - now apply IH.
+Qed.
+
+Lemma pop_state_valid symbols_to_pop stk Hp A action lpred :
+  prefix_pred lpred (state_stack_of_stack stk) ->
+  let stk' := fst (pop symbols_to_pop stk Hp (A:=A) action) in
+  state_valid_after_pop (state_of_stack stk') symbols_to_pop lpred.
+Proof.
+  revert stk Hp A action lpred. induction symbols_to_pop as [|t q IH]=>/=.
+  - intros stk Hp A a lpred Hpp. destruct lpred as [|pred lpred]; constructor.
+    inversion Hpp as [|? lpred' ? pred' Himpl Hpp' eq1 eq2]; subst.
+    specialize (Himpl (state_of_stack stk)).
+    destruct (pred' (state_of_stack stk)) as [] eqn:Heqpred'=>//.
+    destruct stk as [|[]]; simpl in *.
+    + inversion eq2; subst; clear eq2.
+      unfold singleton_state_pred in Heqpred'.
+      now rewrite compare_refl in Heqpred'; discriminate.
+    + inversion eq2; subst; clear eq2.
+      unfold singleton_state_pred in Heqpred'.
+      now rewrite compare_refl in Heqpred'; discriminate.
+  - intros stk Hp A a lpred Hpp. destruct stk as [|[] stk]=>//=.
+    + destruct pop_subproof0.
+    + destruct lpred as [|pred lpred]; [by constructor|].
+      constructor. apply IH. by inversion Hpp.
+Qed.
 
 (** [step_result] represents the result of one step of the automaton : it can
     fail, accept or progress. [Fail_sr] means that the input is incorrect.
@@ -125,62 +213,109 @@ Inductive step_result :=
   | Accept_sr: symbol_semantic_type (NT (start_nt init)) -> Stream token -> step_result
   | Progress_sr: stack -> Stream token -> step_result.
 
-Program Definition prod_action':
-  forall p,
-    arrows_right (symbol_semantic_type (NT (prod_lhs p)))
-      (map symbol_semantic_type (prod_rhs_rev p)):=
-      fun p =>
-        eq_rect _ (fun x => x) (prod_action p) _ _.
-Next Obligation.
-unfold arrows_left, arrows_right; simpl.
-rewrite <- fold_left_rev_right, <- map_rev, rev_involutive.
-reflexivity.
-Qed.
-
 (** [reduce_step] does a reduce action :
    - pops some elements from the stack
    - execute the action of the production
    - follows the goto for the produced non terminal symbol **)
-Definition reduce_step stack_cur production buffer: result step_result :=
-  do (stack_new, sem) <-
-    pop (prod_rhs_rev production) stack_cur (prod_action' production);
-  match goto_table (state_of_stack stack_new) (prod_lhs production) with
-    | Some (exist _ state_new e) =>
+Definition reduce_step stk prod (buffer : Stream token)
+        (Hval : valid_for_reduce (state_of_stack stk) prod)
+        (Hi : stack_invariant stk)
+  : step_result.
+refine
+  ((let '(stk', sem) as ss := pop (prod_rhs_rev prod) stk _ (prod_action prod)
+      return state_valid_after_pop (state_of_stack (fst ss)) _ _ -> _
+    in fun Hval' =>
+    match goto_table (state_of_stack stk') (prod_lhs prod) as goto
+      return (goto = _ -> _) -> _
+    with
+    | Some (exist _ state_new e) => fun _ =>
       let sem := eq_rect _ _ sem _ e in
-      OK (Progress_sr (existT noninitstate_type state_new sem::stack_new) buffer)
-    | None =>
-      match stack_new with
-        | [] =>
-          match compare_eqdec (prod_lhs production) (start_nt init) with
-            | left e =>
-              let sem := eq_rect _ (fun nt => symbol_semantic_type (NT nt)) sem _ e in
-              OK (Accept_sr sem buffer)
-            | right _ => Err
-          end
-        | _::_ => Err
-      end
+      Progress_sr (existT noninitstate_type state_new sem::stk') buffer
+    | None => fun Hval =>
+      let sem := eq_rect _ (fun symb => symbol_semantic_type symb) sem _ _ in
+      Accept_sr sem buffer
+    end (proj2 Hval _ Hval'))
+   (pop_state_valid _ _ _ _ _ _ _)).
+Proof.
+  - clear -Hi Hval.
+    abstract (destruct Hi; eapply prefix_ass; [apply Hval|eassumption]).
+  - clear -Hval. abstract (f_equal; specialize (Hval eq_refl); destruct stk' as [|[]]=>//).
+  - clear -Hi. abstract by destruct Hi.
+Defined.
+
+Lemma reduce_step_stack_invariant_preserved stk prod buffer Hv Hi stk' buffer':
+  reduce_step stk prod buffer Hv Hi = Progress_sr stk' buffer' ->
+  stack_invariant stk'.
+Proof.
+  unfold reduce_step.
+  match goal with
+  | |- context [pop ?symbols_to_pop stk ?Hp ?action] =>
+    assert (Hi':=pop_preserves_invariant symbols_to_pop stk Hp _ action Hi);
+    generalize (pop_state_valid symbols_to_pop stk Hp _ action)
   end.
+  destruct pop as [stk0 sem]=>/=. simpl in Hi'. intros Hv'.
+  assert (Hgoto1:=goto_head_symbs (state_of_stack stk0) (prod_lhs prod)).
+  assert (Hgoto2:=goto_past_state (state_of_stack stk0) (prod_lhs prod)).
+  match goal with | |- context [proj2 Hv ?s ?H] => generalize (proj2 Hv s H) end.
+  destruct goto_table as [[state_new e]|] eqn:EQgoto=>//.
+  intros _ [= <- <-]. constructor=>/=.
+  - constructor. eapply prefix_ass. apply Hgoto1. by destruct Hi'.
+  - unfold state_stack_of_stack; simpl; constructor.
+    + intros ?. by destruct singleton_state_pred.
+    + eapply prefix_pred_ass. apply Hgoto2. by destruct Hi'.
+  - by constructor.
+Qed.
 
 (** One step of parsing. **)
-Definition step stack_cur buffer: result step_result :=
-  match action_table (state_of_stack stack_cur) with
-    | Default_reduce_act production =>
-      reduce_step stack_cur production buffer
-    | Lookahead_act awt =>
-      match Streams.hd buffer with
-        | existT _ term sem =>
-          match awt term with
-            | Shift_act state_new e =>
-              let sem_conv := eq_rect _ symbol_semantic_type sem _ e in
-              OK (Progress_sr (existT noninitstate_type state_new sem_conv::stack_cur)
-                              (Streams.tl buffer))
-            | Reduce_act production =>
-              reduce_step stack_cur production buffer
-            | Fail_action =>
-              OK Fail_sr
-          end
-      end
-  end.
+Definition step stk buffer (Hi : stack_invariant stk): step_result :=
+  match action_table (state_of_stack stk) as a return
+    match a return Prop with
+    | Default_reduce_act prod => _
+    | Lookahead_act awt => _
+    end -> _
+  with
+  | Default_reduce_act prod => fun Hv =>
+    reduce_step stk prod buffer Hv Hi
+  | Lookahead_act awt => fun Hv =>
+    match Streams.hd buffer with
+    | existT _ term sem =>
+      match awt term as a return
+        match a return Prop with Reduce_act p => _ | _ => _ end -> _
+      with
+      | Shift_act state_new e => fun _ =>
+        let sem_conv := eq_rect _ symbol_semantic_type sem _ e in
+        Progress_sr (existT noninitstate_type state_new sem_conv::stk)
+                    (Streams.tl buffer)
+      | Reduce_act prod => fun Hv =>
+        reduce_step stk prod buffer Hv Hi
+      | Fail_act => fun _ =>
+        Fail_sr
+      end (Hv term)
+    end
+  end (reduce_ok _).
+
+Lemma step_stack_invariant_preserved stk buffer Hi stk' buffer':
+  step stk buffer Hi = Progress_sr stk' buffer' ->
+  stack_invariant stk'.
+Proof.
+  unfold step.
+  generalize (reduce_ok (state_of_stack stk))=>Hred.
+  assert (Hshift1 := shift_head_symbs (state_of_stack stk)).
+  assert (Hshift2 := shift_past_state (state_of_stack stk)).
+  destruct action_table as [prod|awt]=>/=.
+  - eauto using reduce_step_stack_invariant_preserved.
+  - destruct (Streams.hd buffer) as [term sem].
+    generalize (Hred term). clear Hred. intros Hred.
+    specialize (Hshift1 term). specialize (Hshift2 term).
+    destruct (awt term) as [state_new e|prod|]=>//.
+    + intros [= <- <-]. constructor=>/=.
+      * constructor. eapply prefix_ass. apply Hshift1. by destruct Hi.
+      * unfold state_stack_of_stack; simpl; constructor.
+        -- intros ?. by destruct singleton_state_pred.
+        -- eapply prefix_pred_ass. apply Hshift2. by destruct Hi.
+      * by constructor.
+    + eauto using reduce_step_stack_invariant_preserved.
+Qed.
 
 (** The parsing use a [nat] parameter [n_steps], so that we do not have to prove
     terminaison, which is difficult. So the result of a parsing is either
@@ -193,22 +328,28 @@ Inductive parse_result :=
   | Timeout_pr: parse_result
   | Parsed_pr: symbol_semantic_type (NT (start_nt init)) -> Stream token -> parse_result.
 
-Fixpoint parse_fix stack_cur buffer n_steps: result parse_result:=
-  match n_steps with
-    | O => OK Timeout_pr
-    | S it =>
-      do r <- step stack_cur buffer;
-      match r with
-        | Fail_sr => OK Fail_pr
-        | Accept_sr t buffer_new => OK (Parsed_pr t buffer_new)
-        | Progress_sr s buffer_new => parse_fix s buffer_new it
-      end
+Fixpoint parse_fix stk buffer n_steps (Hi : stack_invariant stk): parse_result:=
+  match n_steps return _ with
+  | O => Timeout_pr
+  | S it =>
+    match step stk buffer Hi as r
+          return (forall stk' (buffer' : Stream token), r = _ -> _) -> _
+    with
+    | Fail_sr => fun _ => Fail_pr
+    | Accept_sr t buffer_new => fun _ => Parsed_pr t buffer_new
+    | Progress_sr s buffer_new => fun Hi =>
+      parse_fix s buffer_new it (Hi s _ eq_refl)
+    end (step_stack_invariant_preserved _ _ _)
   end.
 
-Definition parse buffer n_steps: result parse_result :=
-  parse_fix [] buffer n_steps.
+Definition parse (buffer : Stream token) (n_steps : nat): parse_result.
+refine
+  (parse_fix [] buffer n_steps _).
+Proof.
+  abstract (repeat constructor; intros; by destruct singleton_state_pred).
+Defined.
 
-End Init.
+End Interpreter.
 
 Arguments Fail_sr [init].
 Arguments Accept_sr [init] _ _.
